# baseURI: http://www.tno.nl/mas4aiDEMO
# imports: http://www.w3.org/2004/02/skos/core
# prefix: mas4aiDEMO

@prefix mas4aiDEMO: <http://www.tno.nl/mas4aiDEMO#> .
@prefix owl: <http://www.w3.org/2002/07/owl#> .
@prefix rdf: <http://www.w3.org/1999/02/22-rdf-syntax-ns#> .
@prefix rdfs: <http://www.w3.org/2000/01/rdf-schema#> .
@prefix skos: <http://www.w3.org/2004/02/skos/core#> .
@prefix xsd: <http://www.w3.org/2001/XMLSchema#> .

<http://www.tno.nl/mas4aiDEMO>
  a owl:Ontology ;
  owl:imports <http://www.w3.org/2004/02/skos/core> ;
  owl:versionInfo "Created with TopBraid Composer" ;
.
mas4aiDEMO:ControlledBy
  a owl:ObjectProperty ;
  rdfs:comment "Relating a robotic arm to a software instruction set controlling a given arm"@en ;
  rdfs:domain mas4aiDEMO:RoboticArm ;
  rdfs:label "Controlled by" ;
  rdfs:range mas4aiDEMO:Software ;
  skos:prefLabel "Controlled by" ;
.
mas4aiDEMO:Joint
  a owl:Class ;
  rdfs:comment "A point around which two beams articulate at a specified speed over a specified range"@en ;
  rdfs:label "Joint" ;
  rdfs:subClassOf owl:Thing ;
  skos:prefLabel "Joint" ;
.
mas4aiDEMO:manualLocation
  a owl:DatatypeProperty ;
  rdfs:comment "The web location of the user manual associated with the used tool"@en ;
  rdfs:domain mas4aiDEMO:Tool ;
  rdfs:label "Manual location" ;
  rdfs:range xsd:anyURI ;
  skos:prefLabel "Manual location" ;
.
mas4aiDEMO:ManufacturingResource
  a owl:Class ;
  rdfs:comment "A generic manufacturing resource which one may encounter in a factory"@en ;
  rdfs:label "Manufacturing Resource" ;
  rdfs:subClassOf owl:Thing ;
  skos:prefLabel "Manufacturing Resource" ;
.
mas4aiDEMO:RoboticArm
  a owl:Class ;
  rdfs:comment "A robot arm which can be used for a variety of different manufacturing tasks depending on the equiped tool"@en ;
  rdfs:label "Robotic Arm" ;
  rdfs:subClassOf mas4aiDEMO:ManufacturingResource ;
  skos:prefLabel "Robotic Arm"@en ;
.
mas4aiDEMO:Software
  a owl:Class ;
  rdfs:comment "The software controlling a robotic arm"@en ;
  rdfs:label "Software" ;
  rdfs:subClassOf owl:Thing ;
  skos:prefLabel "Software" ;
.
mas4aiDEMO:Tool
  a owl:Class ;
  rdfs:comment "A tool which may be used by a robotic arm to have it fullfill a variety of functions"@en ;
  rdfs:label "Tool" ;
  rdfs:subClassOf mas4aiDEMO:ManufacturingResource ;
  skos:prefLabel "Tool" ;
.
mas4aiDEMO:dimensionProperties
  a rdf:Property ;
.
mas4aiDEMO:hasDepth
  a owl:DatatypeProperty ;
  rdfs:comment "The depth of the robotic arm in centimeters"@en ;
  rdfs:domain mas4aiDEMO:RoboticArm ;
  rdfs:label "Has depth" ;
  rdfs:range xsd:integer ;
  rdfs:subPropertyOf mas4aiDEMO:dimensionProperties ;
  skos:prefLabel "Has depth" ;
.
mas4aiDEMO:hasHeight
  a owl:DatatypeProperty ;
  rdfs:comment "The height of the robotic arm, expressed in cm"@en ;
  rdfs:domain mas4aiDEMO:RoboticArm ;
  rdfs:label "Has height" ;
  rdfs:range xsd:integer ;
  rdfs:subPropertyOf mas4aiDEMO:dimensionProperties ;
  skos:prefLabel "Has height" ;
.
mas4aiDEMO:hasJoint
  a owl:ObjectProperty ;
  rdfs:comment "Relating a robotic arm to its joints"@en ;
  rdfs:domain mas4aiDEMO:RoboticArm ;
  rdfs:label "Has joint" ;
  rdfs:range mas4aiDEMO:Joint ;
  skos:prefLabel "Has joint" ;
.
mas4aiDEMO:hasMaxSpeed
  a owl:DatatypeProperty ;
  rdfs:comment "The maximum speed of rotation of a joint, expressed in degrees per second"@en ;
  rdfs:domain mas4aiDEMO:Joint ;
  rdfs:label "Has Maximum speed" ;
  rdfs:range xsd:decimal ;
  skos:prefLabel "Has maximum speed" ;
.
mas4aiDEMO:hasRange
  a owl:DatatypeProperty ;
  rdfs:comment "The range over which a joint can articulate, expressed in the amount of degrees between the two limits of rotation"@en ;
  rdfs:domain mas4aiDEMO:Joint ;
  rdfs:label "Has range" ;
  rdfs:range xsd:decimal ;
  skos:prefLabel "Has range" ;
.
mas4aiDEMO:hasVersionNumber
  a owl:DatatypeProperty ;
  rdfs:comment "The version number of a piece of software"@en ;
  rdfs:domain mas4aiDEMO:Software ;
  rdfs:label "Has version number" ;
  rdfs:range xsd:integer ;
  skos:prefLabel "Has version number" ;
.
mas4aiDEMO:hasWeight
  a owl:DatatypeProperty ;
  rdfs:comment "The weight of a piece of manufacturing equipment, expressed in Kg"@en ;
  rdfs:domain mas4aiDEMO:ManufacturingResource ;
  rdfs:label "Has weight" ;
  rdfs:range xsd:integer ;
  skos:prefLabel "Has weight" ;
.
mas4aiDEMO:hasWidth
  a owl:DatatypeProperty ;
  rdfs:comment "The width of the robotic arm, expressed in cm"@en ;
  rdfs:domain mas4aiDEMO:RoboticArm ;
  rdfs:label "Has width" ;
  rdfs:range xsd:integer ;
  rdfs:subPropertyOf mas4aiDEMO:dimensionProperties ;
  skos:prefLabel "Has width" ;
.
mas4aiDEMO:usesTool
  a owl:ObjectProperty ;
  rdfs:comment "Relates a robotic arm to the tool it is currently equiped with"@en ;
  rdfs:domain mas4aiDEMO:RoboticArm ;
  rdfs:label "Uses tool" ;
  rdfs:range mas4aiDEMO:Tool ;
  skos:prefLabel "Uses tool" ;
.


# Instance
mas4aiDEMO:RoboticArm1 a mas4aiDEMO:RoboticArm ;
  rdfs:label "RoboticArm1" ;
  mas4aiDEMO:hasDepth 50 ;
  mas4aiDEMO:hasHeight 95 ;
  mas4aiDEMO:hasWeight 250 ;
  mas4aiDEMO:hasWidth 50 ;
  mas4aiDEMO:ControlledBy mas4aiDEMO:Software1 ;
  mas4aiDEMO:hasJoint mas4aiDEMO:Joint1 ;
  mas4aiDEMO:usesTool mas4aiDEMO:Tool1 .

mas4aiDEMO:Software1 a mas4aiDEMO:Software ;
  mas4aiDEMO:hasVersionNumber 1 .

mas4aiDEMO:Joint1 a mas4aiDEMO:Joint ;
  mas4aiDEMO:hasMaxSpeed "7"^^xsd:decimal ;
  mas4aiDEMO:hasRange "180"^^xsd:decimal .

mas4aiDEMO:Tool1 a mas4aiDEMO:Tool ;
  mas4aiDEMO:manualLocation "https://www.mas4ai.eu/publications/"^^xsd:anyURI ;
  mas4aiDEMO:hasWeight 2 .